theories/merge_sort.v
@@ -1,3 +1,4 @@
+From stdpp Require Export sorting.
 From iris.base_logic.lib Require Export invariants.
 From iris.heap_lang Require Import array lang proofmode notation par.
 
@@ -12,7 +13,7 @@ From iris.heap_lang Require Import array lang proofmode notation par.
   We merge two arrays a1 and a2 of lengths n1 and n2 into an array b
   of length n1 + n2.
 *)
-Definition merge_inner : val :=
+Definition merge : val :=
   rec: "merge" "a1" "n1" "a2" "n2" "b" :=
   (* If a1 is empty, we simply copy the second a2 into b *)
   if: "n1" = #0 then
@@ -35,116 +36,34 @@ Definition merge_inner : val :=
       "merge" "a1" "n1" ("a2" +ₗ #1) ("n2" - #1) ("b" +ₗ #1).
 
 (*
-  Heaplang recuires array allocations to contain atleast 1 element. So
-  in the case that either of the peaces is empty, we simply return the
-  other.
-*)
-Definition merge : val :=
-  λ: "a1" "n1" "a2" "n2",
-  if: "n1" = #0 then
-    "a2"
-  else if: "n2" = #0 then
-    "a1"
-  else
-    let: "b" := AllocN ("n1" + "n2") #() in
-    merge_inner "a1" "n1" "a2" "n2" "b";;
-    "b".
-
-(*
   To sort we simply split the array in half. Sort them on seperate
-  threads. Then the results are merged together.
+  threads. Then the results are merged together and copied back into the array.
 *)
-Definition merge_sort : val :=
-  rec: "merge_sort" "a" "n" :=
-  if: "n" ≤ #1 then
-    "a"
+Definition merge_sort_inner : val :=
+  rec: "merge_sort_inner" "a" "b" "n" :=
+  if: "n" ≤ #1 then #()
   else
     let: "n1" := "n" `quot` #2 in
     let: "n2" := "n" - "n1" in
-    let: "p" := ("merge_sort" "a" "n1" ||| "merge_sort" ("a" +ₗ "n1") "n2") in
-    merge (Fst "p") "n1" (Snd "p") "n2".
+    ("merge_sort_inner" "b" "a" "n1" ||| "merge_sort_inner" ("b" +ₗ "n1") ("a" +ₗ "n1") "n2");;
+    merge "b" "n1" ("b" +ₗ "n1") "n2" "a".
+
+(*
+  Heaplang recuires array allocations to contain atleast 1 element. So
+  we need to treat this case seperatly.
+*)
+Definition merge_sort : val :=
+  λ: "a" "n",
+  if: "n" = #0 then #()
+  else
+    let: "b" := AllocN "n" #() in
+    array_copy_to "b" "a" "n";;
+    merge_sort_inner "a" "b" "n".
 
 (*
   Our desired specification will be that sort produces a new sorted
   array that's a permutation of the input.
-
-  We define sorting as follows:
 *)
-Inductive sorted : list Z → Prop :=
-  | sorted_nil : sorted []
-  | sorted_singleton x : sorted [x]
-  | sorted_cons_cons x y l : (x ≤ y)%Z → sorted (y :: l) → sorted (x :: y :: l).
-
-(*
-  Alternatively a list is sorted if all ordered pairs of indecies
-  corresponds to orderered values.
-*)
-Lemma sorted_alt l : sorted l ↔ ∀ i j x y, l !! i = Some x → l !! j = Some y → i ≤ j → (x ≤ y)%Z.
-Proof.
-  split.
-  - induction 1 as [|x|x y l H Hl IH].
-    + intros i j x y H.
-      done.
-    + intros i j y z Hi Hj _.
-      apply list_lookup_singleton_Some in Hi.
-      apply list_lookup_singleton_Some in Hj.
-      destruct Hi as [-> <-].
-      destruct Hj as [-> <-].
-      done.
-    + intros i j z w Hi Hj Hle.
-      destruct i, j; cbn in Hi, Hj.
-      -- injection Hi as <-.
-        injection Hj as <-.
-        done.
-      -- injection Hi as <-.
-        trans y=>//.
-        apply (IH 0 j)=>//.
-        apply le_0_n.
-      -- inversion Hle.
-      -- by apply (IH i j), le_S_n.
-  - intros H.
-    induction l as [|x [|y l] IH].
-    all: constructor.
-    + apply (H 0 1)=>//.
-      by constructor.
-    + apply IH => i j z w Hi Hj Hle.
-      by apply (H (S i) (S j)), le_n_S.
-Qed.
-
-Lemma sorted_cons x l : sorted (x :: l) ↔ sorted l ∧ ∀ y, y ∈ l → (x ≤ y)%Z.
-Proof.
-  rewrite !sorted_alt.
-  split.
-  - intros H.
-    split.
-    + intros i j y z Hi Hj Hle.
-      by apply (H (S i) (S j)), le_n_S.
-    + intros y Hy.
-      apply elem_of_list_lookup in Hy.
-      destruct Hy as [i Hi].
-      by apply (H 0 (S i)), le_0_n.
-  - intros [H H0] i j y z Hi Hj Hle.
-    destruct i, j; cbn in *.
-    + injection Hi as <-.
-      injection Hj as <-.
-      done.
-    + injection Hi as <-.
-      apply H0, elem_of_list_lookup.
-      by exists j.
-    + inversion Hle.
-    + by apply (H i j), le_S_n.
-Qed.
-
-Lemma sorted_le_1 l : length l ≤ 1 → sorted l.
-Proof.
-  intros H.
-  destruct l as [|x [|y l]].
-  - apply sorted_nil.
-  - apply sorted_singleton.
-  - contradict H.
-    apply Nat.lt_nge=>/=.
-    apply le_n_S, le_n_S, le_0_n.
-Qed.
 
 Section proofs.
 Context `{!heapGS Σ, !spawnG Σ}.
@@ -154,32 +73,28 @@ Context `{!heapGS Σ, !spawnG Σ}.
   sorted. Furthermore we need the result array b to have enough space,
   though we don't care what it contains.
 *)
-Lemma merge_inner_spec (a1 a2 b : loc) (l1 l2 : list Z) (l : list val) :
-  {{{a1 ↦∗ ((λ x : Z, #x) <$> l1) ∗ a2 ↦∗ ((λ x : Z, #x) <$> l2) ∗ b ↦∗ l ∗ ⌜sorted l1⌝ ∗ ⌜sorted l2⌝ ∗ ⌜length l = (length l1 + length l2)%nat⌝}}}
-    merge_inner #a1 #(length l1) #a2 #(length l2) #b
-  {{{(l : list Z), RET #(); b ↦∗ ((λ x : Z, #x) <$> l) ∗ ⌜sorted l⌝ ∗ ⌜l1 ++ l2 ≡ₚ l⌝}}}.
-Proof.
-  iIntros "%Φ (Ha1 & Ha2 & Hb & %Hl1 & %Hl2 & %H) HΦ".
-  iLöb as "IH" forall (a1 a2 b l1 l2 l Hl1 Hl2 H).
-  (* FILL IN HERE *) Admitted.
-
-Lemma merge_spec (a1 a2 : loc) (l1 l2 : list Z) :
-  {{{a1 ↦∗ ((λ x : Z, #x) <$> l1) ∗ a2 ↦∗ ((λ x : Z, #x) <$> l2) ∗ ⌜sorted l1⌝ ∗ ⌜sorted l2⌝}}}
-    merge #a1 #(length l1) #a2 #(length l2)
-  {{{(b : loc) (l : list Z), RET #b; b ↦∗ ((λ x : Z, #x) <$> l) ∗ ⌜sorted l⌝ ∗ ⌜l1 ++ l2 ≡ₚ l⌝}}}.
+Lemma merge_spec (a1 a2 b : loc) (l1 l2 : list Z) (l : list val) :
+  {{{a1 ↦∗ ((λ x : Z, #x) <$> l1) ∗ a2 ↦∗ ((λ x : Z, #x) <$> l2) ∗ b ↦∗ l ∗ ⌜StronglySorted Z.le l1⌝ ∗ ⌜StronglySorted Z.le l2⌝ ∗ ⌜length l = (length l1 + length l2)%nat⌝}}}
+    merge #a1 #(length l1) #a2 #(length l2) #b
+  {{{(l : list Z), RET #(); a1 ↦∗ ((λ x : Z, #x) <$> l1) ∗ a2 ↦∗ ((λ x : Z, #x) <$> l2) ∗ b ↦∗ ((λ x : Z, #x) <$> l) ∗ ⌜StronglySorted Z.le l⌝ ∗ ⌜l1 ++ l2 ≡ₚ l⌝}}}.
 Proof.
   (* FILL IN HERE *) Admitted.
 
 (*
-  With this we can finally prove that sort actually sorts the output.
+  With this we can prove that sort actually sorts the output.
 *)
+Lemma merge_sort_inner_spec (a b : loc) (l : list Z) :
+  {{{a ↦∗ ((λ x : Z, #x) <$> l) ∗ b ↦∗ ((λ x : Z, #x) <$> l)}}}
+    merge_sort_inner #a #b #(length l)
+  {{{(l' : list Z) vs, RET #(); a ↦∗ ((λ x : Z, #x) <$> l') ∗ b ↦∗ vs ∗ ⌜StronglySorted Z.le l'⌝ ∗ ⌜l ≡ₚ l'⌝ ∗ ⌜length vs = length l'⌝}}}.
+Proof.
+  (* FILL IN HERE *) Admitted.
+
 Lemma merge_sort_spec (a : loc) (l : list Z) :
   {{{a ↦∗ ((λ x : Z, #x) <$> l)}}}
     merge_sort #a #(length l)
-  {{{(b : loc) (l' : list Z), RET #b; b ↦∗ ((λ x : Z, #x) <$> l') ∗ ⌜sorted l'⌝ ∗ ⌜l ≡ₚ l'⌝}}}.
+  {{{(l' : list Z), RET #(); a ↦∗ ((λ x : Z, #x) <$> l') ∗ ⌜StronglySorted Z.le l'⌝ ∗ ⌜l ≡ₚ l'⌝}}}.
 Proof.
-  iIntros "%Φ Ha HΦ".
-  iLöb as "IH" forall (a l Φ).
   (* FILL IN HERE *) Admitted.
 
 End proofs.
